WIP: SIM2

dataplane/Examples/Ooo_Input_op.thy
@@ -41,6 +41,128 @@ definition ooo_input_os_Drop_Mint where
     Drop t \<Rightarrow> drop_cap os (Cap t p)
   | Mint t \<Rightarrow> add_cap os p t)\<close>
 
+
+fun ocaps_updates where
+  "ocaps_updates caps [] = caps"
+| "ocaps_updates caps ((Data t d) # xs) = ocaps_updates caps xs"
+| "ocaps_updates caps ((Drop t) # xs) = ocaps_updates (remove_last t caps) xs"
+| "ocaps_updates caps ((Mint t) # xs) = ocaps_updates (caps @ [t]) xs"
+
+lemma ooo_input_op_logic_iterates_n:
+  "ocaps os p \<noteq> [] \<Longrightarrow>
+   p |\<in>| P \<Longrightarrow>
+   llength (es os p) \<ge> enat n \<Longrightarrow>
+   os\<lparr>es := (es os)( p := ldropn n (es os p)),
+      ocaps := (ocaps os)(p := ocaps_updates (ocaps os p) (ltaken n (es os p))),
+      inter := inter os @ (map (\<lambda> ev. case ev of Drop t \<Rightarrow> (p, t, -1) | Mint t \<Rightarrow> (p, t, 1)) (filter (Not o is_Data) (ltaken n (es os p)))),
+      produ := produ os @ (map (\<lambda> ev. case ev of Data t d \<Rightarrow> (p, t, 1)) (filter is_Data (ltaken n (es os p)))),
+      outpu := (outpu os)( p := outpu os p @ (map (\<lambda> ev. case ev of Data t d \<Rightarrow> (en1 os d, t)) (filter is_Data (ltaken n (es os p)))) ) \<rparr> |\<in>|
+   ((\<lambda>oss. cUnion (ooo_input_op_logic P |`| oss)) ^^ n) {|os|}"
+  apply (induct n arbitrary: os rule: less_induct)
+  subgoal for n os
+    apply (cases n)
+    subgoal
+      by simp
+    subgoal for n'
+      apply (cases "es os p"; simp add: zero_enat_def flip: cin.rep_eq )
+    subgoal for ev lxs
+      apply (cases ev)
+      subgoal for t d
+        apply (clarsimp simp flip: cin.rep_eq)
+        apply (cases n')
+        subgoal
+        apply (clarsimp simp flip: cin.rep_eq)
+           apply simp_all
+          unfolding ooo_input_op_logic_def produce_def
+          apply (clarsimp simp add: image_iff simp flip: cin.rep_eq)
+          apply (rule exI[of _ p])
+          apply simp
+          done
+        subgoal for n''
+          apply (clarsimp simp add: image_iff simp flip: cin.rep_eq)
+          apply hypsubst_thin
+          subgoal premises prems
+            apply (rule cBexI[rotated])
+            apply (simp add: cUNION_cimage flip: cin.rep_eq)
+            apply (rule cBexI[rotated])
+              apply (rule prems(1))
+            using prems(2-) apply simp
+            using prems(2-) apply simp
+            subgoal
+           using prems(2-) by (metis Suc_ile_eq llength_LCons nless_le)
+           apply (subst ooo_input_op_logic_def)
+          using prems(2-) apply -
+           apply (simp add: cUNION_cimage flip: cin.rep_eq)
+          apply (rule exI[of _ p])
+           apply (simp add: cUNION_cimage flip: cin.rep_eq)
+           apply (intro conjI)
+            defer
+            apply (rule refl)
+           apply (clarsimp simp add: cUNION_cimage flip: cin.rep_eq split: llist.splits)
+
+            find_theorems "cUnion ( _ |`| _) = _"
+
+
+
+            find_theorems "_ |\<in>| cfilter _ _"
+
+end
+
+
+    apply (drule meta_spec[of _ "os\<lparr> es := (es os)(p := ltl (es os p)), produ := produ os @ [(p, t, 1)], outpu := (outpu os)( p := outpu os p @ [(en1 os d, t)]) \<rparr>"])
+    apply simp
+    apply (drule meta_mp)
+    subgoal
+      apply (metis eSuc_enat eSuc_ile_mono)
+      done
+    subgoal
+      apply (clarsimp simp flip: cin.rep_eq)
+
+
+
+end
+      apply (rule exI[of _ "os\<lparr>es := (es os)(p := ldropn n lxs), ocaps := (ocaps os)(p := ocaps_updates (ocaps os p) (ltaken n lxs)),
+         inter := operator_state.inter os @ map (case_event (\<lambda>a aa. undefined) (\<lambda>t. (p, t, - 1)) (\<lambda>t. (p, t, 1))) (filter (Not \<circ> is_Data) (ltaken n lxs)),
+         produ := produ os @ (p, t, 1) # map (case_event (\<lambda>t d. (p, t, 1)) (\<lambda>a. undefined) (\<lambda>a. undefined)) (filter is_Data (ltaken n lxs)),
+         outpu := (outpu os)(p := outpu os p @ (en1 os d, t) # map (case_event (\<lambda>t d. (en1 os d, t)) (\<lambda>a. undefined) (\<lambda>a. undefined)) (filter is_Data (ltaken n lxs)))\<rparr>"])
+      subgoal
+        apply (intro conjI)
+        subgoal premises temp
+          using temp(7) apply -
+          apply (cases n)
+          subgoal
+        unfolding ooo_input_op_logic_def drop_caps_def
+        apply (auto simp flip: cin.rep_eq split: event.splits llist.splits)
+
+
+end
+      apply (rule exI[of _ "os\<lparr>es := (es os)(p := ldropn n (ltl (es os p)))\<rparr>"])
+      apply (clarsimp simp flip: cin.rep_eq)
+      apply (intro conjI[rotated])
+      subgoal premises temp
+        using temp(1,2,3,4) apply -
+        unfolding ooo_input_op_logic_def drop_caps_def
+        apply (auto simp flip: cin.rep_eq split: event.splits llist.splits)
+        apply (intro exI conjI impI)
+             defer
+             apply assumption+
+           apply simp
+        subgoal
+          by simp
+        subgoal
+          apply auto
+          subgoal
+            
+
+
+
+end
+    apply (auto simp flip: cin.rep_eq split: event.splits llist.splits)
+    apply (rule cBexI[rotated])
+    apply (simp flip: cin.rep_eq)
+
+    find_theorems "_ |\<in>| cfilter _ _"
+
 (* record ('p, 'd, 'd1, 'd2, 'd3, 't) input_state_ty3 = "('p, 'd, 'd1, 'd2, 't) input_state2" +  es3:: "('t, 'd3) event llist"
 
 definition ooo_input_ty3_op where
