dataplane/Correctness/Outputs.thy
@@ -20,7 +20,7 @@ lemma dataplane_tracker_inv_update_outputs_outside:
   apply hypsubst_thin
   subgoal for caps
     apply (rule exI[of _ caps])
-    apply (intro conjI)
+    apply (intro conjI)                                         
     subgoal premises prems
       using prems(3) apply -
       unfolding Src_caps_inv_def
@@ -33,7 +33,7 @@ lemma dataplane_tracker_inv_update_outputs_outside:
       apply (rule arg_cong[where f=to_zmset])
       apply (rule map_cong)
       unfolding BULK_BENQ_def
-       apply (auto split: prod.splits)
+      apply (auto split: prod.splits)
       subgoal for nid' p' nid'' p''
         apply (cases "nid'' = nid \<and> p'' = p")
         subgoal
@@ -58,10 +58,10 @@ lemma dataplane_tracker_inv_update_outputs_outside:
           apply (simp add:  c_pts_change_multiplicities)
           apply (rule arg_cong[where f=zmset])
           apply (rule map_cong)
-           apply (rule filter_cong)
-            apply (rule arg_cong[where f=concat])
-            apply (rule map_cong)
-             apply auto
+          apply (rule filter_cong)
+          apply (rule arg_cong[where f=concat])
+          apply (rule map_cong)
+          apply auto
           done
         done
       done
@@ -92,23 +92,23 @@ lemma dataplane_tracker_inv_update_outputs_outside:
       subgoal for xs a b c
         apply (drule spec2)
         apply (drule mp)
-         apply assumption
+        apply assumption
         apply (drule mp)
-         apply assumption
+        apply assumption
         apply (drule bspec)
         unfolding extract_progress_def obtain_progress_def
-         apply simp
+        apply simp
         apply auto
         done
       subgoal for xs' a b c
         apply (drule spec2)
         apply (drule mp)
-         apply assumption
+        apply assumption
         apply (drule mp)
-         apply assumption
+        apply assumption
         apply (drule bspec)
         unfolding extract_progress_def obtain_progress_def
-         apply simp
+        apply simp
         apply clarsimp
         apply (subgoal_tac "extract_prog a (subgraph.nxt sg) (map_entry nid (outpu_update (\<lambda>_ p'. if p' = p then xs else outpu (os nid) p')) os) = extract_prog a (subgraph.nxt sg) os")
         subgoal
@@ -118,7 +118,7 @@ lemma dataplane_tracker_inv_update_outputs_outside:
           apply clarsimp
           apply (rule arg_cong[where f=concat])
           apply (rule map_cong)
-           apply auto
+          apply auto
           done
         done
       done
@@ -134,7 +134,7 @@ lemma dataplane_tracker_inv_update_outputs_outside:
           by auto
         subgoal premises temp
           apply (rule map_cong)
-           apply auto
+          apply auto
           done
         done
       subgoal for p'' t m
@@ -145,7 +145,7 @@ lemma dataplane_tracker_inv_update_outputs_outside:
           by auto
         subgoal premises temp
           apply (rule map_cong)
-           apply auto
+          apply auto
           done
         done
       done
@@ -190,13 +190,13 @@ lemma dataplane_tracker_inv_update_outputs:
       apply clarsimp
       apply (rule arg_cong[where f=to_zmset])
       apply (rule map_cong)
-       apply simp_all
+      apply simp_all
       unfolding BULK_BENQ_def
       apply (auto split: prod.splits)
       subgoal 
         apply (drule the_elem_graph_summar_nt_summ[OF _ prems(3)])
-         back
-         apply assumption
+        back
+        apply assumption
         apply clarsimp
         apply (rule FalseE)
         using conjunct1[OF conjunct2[OF conjunct2[OF conjunct2[OF conjunct2[OF conjunct2[OF conjunct2[OF prems(3)[unfolded graph_summar_nt_def]]]]]]]]
@@ -206,8 +206,8 @@ lemma dataplane_tracker_inv_update_outputs:
         done
       subgoal 
         apply (drule the_elem_graph_summar_nt_summ[OF _ prems(3)])
-         back
-         apply assumption
+        back
+        apply assumption
         apply clarsimp
         apply (rule FalseE)
         using conjunct1[OF conjunct2[OF conjunct2[OF conjunct2[OF conjunct2[OF conjunct2[OF conjunct2[OF prems(3)[unfolded graph_summar_nt_def]]]]]]]]
@@ -217,8 +217,8 @@ lemma dataplane_tracker_inv_update_outputs:
         done
       subgoal 
         apply (drule the_elem_graph_summar_nt_summ[OF _ prems(3)])
-         back
-         apply assumption
+        back
+        apply assumption
         apply clarsimp
         apply (rule FalseE)
         using conjunct1[OF conjunct2[OF conjunct2[OF conjunct2[OF conjunct2[OF conjunct2[OF conjunct2[OF prems(3)[unfolded graph_summar_nt_def]]]]]]]]
@@ -228,8 +228,8 @@ lemma dataplane_tracker_inv_update_outputs:
         done
       subgoal 
         apply (drule the_elem_graph_summar_nt_summ[OF _ prems(3)])
-         back
-         apply assumption
+        back
+        apply assumption
         apply clarsimp
         apply (rule FalseE)
         using conjunct1[OF conjunct2[OF conjunct2[OF conjunct2[OF conjunct2[OF conjunct2[OF conjunct2[OF prems(3)[unfolded graph_summar_nt_def]]]]]]]]
@@ -271,10 +271,10 @@ lemma dataplane_tracker_inv_update_outputs:
           apply (simp add:  c_pts_change_multiplicities)
           apply (rule arg_cong[where f=zmset])
           apply (rule map_cong)
-           apply (rule filter_cong)
-            apply (rule arg_cong[where f=concat])
-            apply (rule map_cong)
-             apply auto
+          apply (rule filter_cong)
+          apply (rule arg_cong[where f=concat])
+          apply (rule map_cong)
+          apply auto
           done
         done
       done
@@ -296,9 +296,9 @@ lemma dataplane_tracker_inv_update_outputs:
         apply (auto 0 0 simp add: image_iff split: prod.splits if_splits)
         subgoal
           apply (drule the_elem_graph_summar_nt_summ[OF _ prems(3)])
-           apply assumption
+          apply assumption
           apply (drule the_elem_graph_summar_nt_summ[OF _ prems(3)])
-           apply assumption
+          apply assumption
           apply clarsimp
           using conjunct1[OF conjunct2[OF conjunct2[OF conjunct2[OF conjunct2[OF conjunct2[OF conjunct2[OF prems(3)[unfolded graph_summar_nt_def]]]]]]]]
             the_elem_bi_unique_op_conn
@@ -307,9 +307,9 @@ lemma dataplane_tracker_inv_update_outputs:
           done
         subgoal
           apply (drule the_elem_graph_summar_nt_summ[OF _ prems(3)])
-           apply assumption
+          apply assumption
           apply (drule the_elem_graph_summar_nt_summ[OF _ prems(3)])
-           apply assumption
+          apply assumption
           apply clarsimp
           using conjunct1[OF conjunct2[OF conjunct2[OF conjunct2[OF conjunct2[OF conjunct2[OF conjunct2[OF prems(3)[unfolded graph_summar_nt_def]]]]]]]]
             the_elem_bi_unique_op_conn
@@ -318,40 +318,40 @@ lemma dataplane_tracker_inv_update_outputs:
           done
         subgoal
           apply (drule the_elem_graph_summar_nt_summ[OF _ prems(3)])
-           apply assumption
+          apply assumption
           apply (drule the_elem_graph_summar_nt_summ[OF _ prems(3)])
-           apply assumption
+          apply assumption
           apply clarsimp
           done
         subgoal
           apply (drule the_elem_graph_summar_nt_summ[OF _ prems(3)])
-           apply assumption
+          apply assumption
           apply (drule the_elem_graph_summar_nt_summ[OF _ prems(3)])
-           apply assumption
+          apply assumption
           apply clarsimp
           done
         subgoal
           apply (drule the_elem_graph_summar_nt_summ[OF _ prems(3)])
-           apply assumption
+          apply assumption
           apply clarsimp
           done
         subgoal
           apply (drule the_elem_graph_summar_nt_summ[OF _ prems(3)])
-           apply assumption
+          apply assumption
           apply (drule the_elem_graph_summar_nt_summ[OF _ prems(3)])
-           apply assumption
+          apply assumption
           apply clarsimp
           done
         subgoal
           apply (drule the_elem_graph_summar_nt_summ[OF _ prems(3)])
-           apply assumption
+          apply assumption
           apply (drule the_elem_graph_summar_nt_summ[OF _ prems(3)])
-           apply assumption
+          apply assumption
           apply clarsimp
           done
         subgoal
           apply (drule the_elem_graph_summar_nt_summ[OF _ prems(3)])
-           apply assumption
+          apply assumption
           apply clarsimp
           done
         done
@@ -368,23 +368,23 @@ lemma dataplane_tracker_inv_update_outputs:
       subgoal for xs 
         apply (drule spec2)
         apply (drule mp)
-         apply assumption
+        apply assumption
         apply (drule mp)
-         apply assumption
+        apply assumption
         apply (drule bspec)
         unfolding extract_progress_def obtain_progress_def
-         apply simp
+        apply simp
         apply auto
         done
       subgoal for xs' a b c
         apply (drule spec2)
         apply (drule mp)
-         apply assumption
+        apply assumption
         apply (drule mp)
-         apply assumption
+        apply assumption
         apply (drule bspec)
         unfolding extract_progress_def obtain_progress_def
-         apply simp
+        apply simp
         apply clarsimp
         apply (subgoal_tac "extract_prog a (subgraph.nxt sg) (map_entry nid (outpu_update (\<lambda>_ p'. if p' = p then ys else outpu (os nid) p')) os) = extract_prog a (subgraph.nxt sg) os")
         subgoal
@@ -394,7 +394,7 @@ lemma dataplane_tracker_inv_update_outputs:
           apply clarsimp
           apply (rule arg_cong[where f=concat])
           apply (rule map_cong)
-           apply auto
+          apply auto
           done
         done
       done
@@ -414,7 +414,7 @@ lemma dataplane_tracker_inv_update_outputs:
           by auto
         subgoal premises temp
           apply (rule map_cong)
-           apply auto
+          apply auto
           done
         done
       subgoal for nid'' p'' t'' m
@@ -428,7 +428,7 @@ lemma dataplane_tracker_inv_update_outputs:
           by auto
         subgoal premises temp
           apply (rule map_cong)
-           apply auto
+          apply auto
           done
         done
       done
